src/opt/ReorderStore.v
@@ -118,7 +118,7 @@ Lemma sim_store_future
       (MEM1: sim_memory mem1_src mem1_tgt)
       (SIM1: sim_store st_src lc_src sc1_src mem1_src
                        st_tgt lc_tgt sc1_tgt mem1_tgt)
-      (CONCRETE_SRC: Memory.concrete_exact mem1_src mem2_src)
+      (CONCRETE_SRC: Memory.concrete mem1_src mem2_src)
       (WF_SRC: Local.wf lc_src mem2_src)
       (MEM_SRC: Memory.closed mem2_src)
       (NOHALF_SRC: Memory.no_half lc_src.(Local.promises) mem2_src):
@@ -126,7 +126,7 @@ Lemma sim_store_future
     <<MEM2: sim_memory mem2_src mem2_tgt>> /\
     <<FUTURE_SRC: Memory.future mem1_src mem2_src>> /\
     <<FUTURE_TGT: Memory.future mem1_tgt mem2_tgt>> /\
-    <<CONCRETE_TGT: Memory.concrete_exact mem1_tgt mem2_tgt>> /\
+    <<CONCRETE_TGT: Memory.concrete mem1_tgt mem2_tgt>> /\
     <<WF_TGT: Local.wf lc_tgt mem2_tgt>> /\
     <<MEM_TGT: Memory.closed mem2_tgt>> /\
     <<HALF_WF_SRC: Memory.half_wf mem2_src>> /\
@@ -136,7 +136,7 @@ Lemma sim_store_future
                       st_tgt lc_tgt sc1_tgt mem2_tgt>>.
 Proof.
   inv SIM1.
-  exploit Memory.no_half_concrete_exact_future;
+  exploit Memory.no_half_concrete_future;
     try exact CONCRETE_SRC; try apply WF_SRC; try apply WF_SRC0; eauto. i.
   exploit fulfill_step_future; eauto; try by viewtac. i. des.
   exploit fulfill_step_future; try exact WF_SRC;
@@ -153,7 +153,7 @@ Proof.
   exploit SimPromises.concrete_future;
     [exact CONCRETE_SRC|exact CONCRETE_TGT|..]; eauto. i. des.
   esplits; eauto.
-  econs; eauto using Memory.concrete_exact_closed_timemap.
+  econs; eauto using Memory.concrete_closed_timemap.
 Qed.
 
 Lemma sim_store_step
