src/opt/SimMemory.v
@@ -578,9 +578,9 @@ Proof.
   inv TGT; ss. econs. eapply sim_memory_closed_opt_view; eauto.
 Qed.
 
-Lemma concrete_exact_covered
+Lemma concrete_covered
       mem1 mem2 loc ts
-      (CONCRETE: Memory.concrete_exact mem1 mem2):
+      (CONCRETE: Memory.concrete mem1 mem2):
   covered loc ts mem1 <-> covered loc ts mem2.
 Proof.
   inv CONCRETE. split; i.
